scheduler.dfy
@@ -1,0 +1,117 @@
+// Implements scheduler with the TreeQueue class.
+
+class {:autocontracts} Node
+{
+  var state: State;
+  var pc: SatLib.BoolExpr;
+  constructor (input_state: State, input_pc: SatLib.BoolExpr)
+  {
+    state, pc := input_state, input_pc;
+  }
+}
+datatype NodeMaybe = Some(v:Node) | None
+
+// TreeQueue
+// Stores a tree where each node contains a state and the path condition
+// that leads to that state. When a state only has one possible next
+// state, the node will be NodeMaybe.None, otherwise in will be
+// Some(Node).
+//
+// The enqueue operations assign children to the last dequeued node. All
+// children of a dequeued node should be enqueued before the next item
+// is dequeued.
+//
+// Alternate array-base queue implementation found in:
+//   "Developing Verified Programs with Dafny", figure 4.
+//   https://www.microsoft.com/en-us/research/wp-content/uploads/2016/12/krml233.pdf
+class {:autocontracts} TreeQueue
+{
+
+  // Stores tree for states and path condition
+  var a: array<NodeMaybe>;
+
+  // Indexes into "a".
+  // start points to the next node to be dequeued.
+  // end points to the highest non-None node in the tree.
+  var start: int, end: int;
+
+  predicate Valid() {
+    (a != null) && (0 <= start <= end < a.Length) && a.Length > 1
+  }
+
+  constructor ()
+  {
+    a, start, end := new NodeMaybe[10], 0, 0;
+  }
+
+  method getTree() returns (T: array<NodeMaybe>)
+  {
+    T := new NodeMaybe[a.Length];
+    T := a;
+  }
+
+  method DoubleEnqueue(lc: Node, rc: Node)
+    ensures 0 <= 2*start + 2 < a.Length
+    ensures match a[2*start + 1]
+        case Some(n) => n == lc
+        case None => false
+    ensures match a[2*start + 2]
+        case Some(node) => node == rc
+        case None => false
+  {
+
+    var b := new NodeMaybe[2*(a.Length+1)-1];
+    assert a.Length < b.Length;
+
+    // Copy a to b
+    forall i | 0 <= i < a.Length < b.Length
+    {
+      b[i] := a[i];
+    }
+    assert forall k :: 0 <= k < a.Length < b.Length ==> a[k] == b[k];
+
+    b[2*start + 1]:= NodeMaybe.Some(lc);
+    b[2*start + 2]:= NodeMaybe.Some(rc);
+    a, end := b, 2*start + 2;
+  }
+  
+  method LeftEnqueue(d: Node)
+    ensures a[2*(start-1)+1] == NodeMaybe.Some(d);
+    ensures a[2*(start-1)+2] == NodeMaybe.None;
+  {
+    var b := new NodeMaybe[3 * a.Length];
+    b := a;
+    b[2*(start-1)+1]:= NodeMaybe.Some(d);
+    b[2*(start-1)+2]:= NodeMaybe.None;
+    a, end := b, 2*(start-1)+1;
+  }
+  
+  method RightEnqueue(d: Node)
+    ensures a[2*(start-1)+1] == NodeMaybe.None;
+    ensures a[2*(start-1)+2] == NodeMaybe.Some(d);
+  {
+    var b := new NodeMaybe[3 * a.Length];
+    b := a;
+    b[2*(start-1)+1]:= NodeMaybe.None;
+    b[2*(start-1)+2]:= NodeMaybe.Some(d);
+    a, end := b, 2*(start-1)+2;
+  }
+  
+  method Dequeue() returns (d: Node)
+    ensures a[start] == a[old(start)+1];
+  {
+    start := start+1;
+    d := match a[start] case Some(node) => node;
+  }
+  
+  function method isEmpty(): bool
+    ensures isEmpty() ==> forall i :: end < i <= a.Length ==> a[i].None?
+  { 
+    a[end] == NodeMaybe.None
+  } 
+}
+
+function method isLeaf(nodeIndex: int, tree:array<Node>): bool
+{
+  (tree[2*nodeIndex+1] == null) && (tree[2*nodeIndex+2] == null)
+}
